prova pendente

Fad/Chapter5-Ex.lean
@@ -1,5 +1,6 @@
 import Fad.Chapter5
 import Fad.Chapter1
+import Mathlib.tactic
 
 namespace Chapter5
 
@@ -19,11 +20,11 @@ example (xs : List Nat) : qsort₀ xs = qsort₁ xs := by
      unfold Tree.flatten
      rfl
   | cons x xs ih =>
-    simp [qsort₀, qsort₁]
-    sorry
+    simp [qsort₀, qsort₁, Function.comp]
+    rw [←ih]
 
 
-/- 5.8 : see book -/
+/- # Exercicio 5.8 : see book -/
 
 
 /- # Exercicio 5.9 -/
@@ -91,32 +92,54 @@ namespace S53
 
 def split [Inhabited a] [LE a] [DecidableRel (α := a) (· ≤ ·)]
  : List a → (a × List a × List a)
+ | []      => (default, [], [])
  | x :: xs =>
    let op x acc :=
     if x ≤ acc.1
     then (x, acc.1 :: acc.2.2, acc.2.1)
     else (acc.1, x :: acc.2.2, acc.2.1)
    xs.foldr op (x, [], [])
- | _      => (default, [], [])
 
-#eval split ([1,2,3,4,5] : List Nat)
+/-- Nn `split₁` the `where` makes `op` visible from outside.
+    In `split`, `let` is defined only in the second equation of
+    the pattern match. `let rec` would make `op` also visible.
+
+    If `op` is not visible, in the `split_left_le` we would need
+    `lift_lets ; intro op` -/
+
+def split₁ [Inhabited a] [LE a] [DecidableRel (α := a) (· ≤ ·)]
+ : List a → (a × List a × List a)
+ | []      => (default, [], [])
+ | x :: xs =>
+   xs.foldr op (x, [], [])
+ where op x acc :=
+  if x ≤ acc.1
+  then (x, acc.1 :: acc.2.2, acc.2.1)
+  else (acc.1, x :: acc.2.2, acc.2.1)
+
+#eval split₁ [3,1,2,4,5]
 
 theorem split_left_le [Inhabited a] [LE a] [DecidableRel (α := a) (· ≤ ·)]
- (xs : List a) : (split xs).2.1.length ≤ xs.length := by
-  induction xs with
-  | nil => simp [split]
-  | cons x xs ih =>
-    have h : (split xs).2.1.length ≤ xs.length := ih
-    -- rw [split]
+ (xs : List a) : (split₁ xs).2.1.length ≤ xs.length := by
+  unfold split₁
+  split
+  . simp
+  . rename_i x xs
+    induction xs with
+    | nil => simp [split]
+    | cons y xs ih =>
+      unfold List.foldr
+      simp [split₁.op]
+      split ; simp
+      rename_i h2
+      sorry
 
-
-def mkHeap [Inhabited a] [LE a] [DecidableRel (α := a) (· ≤ ·)]
+partial def mkHeap [Inhabited a] [LE a] [DecidableRel (α := a) (· ≤ ·)]
  : List a → Tree a
  | []      => Tree.null
  | x :: xs =>
    let p := split (x :: xs)
    Tree.node p.1 (mkHeap p.2.1) (mkHeap p.2.2)
-termination_by xs => xs.length
 
 end S53
 
@@ -155,11 +178,8 @@ def string_incresing_order : Nat → List (String → Char)
   | sz => ((List.range sz).map (fun x => flip String.get ⟨x⟩))
 
 
-def names := ["carlos", "felipe", "mariana", "pedro", "bianca", "gustavo", "camila", "ricardo", "leticia", "renato"]
-
-#eval string_rsort (string_incresing_order 3) ["abc", "def", "ghi", "acb", "dfe", "gih"]
-#eval string_rsort (string_incresing_order 4) ["ac", "deyz", "deyx", "def", "g", "za", "z", "acb", "dfe", "gih"]
-#eval string_rsort (string_incresing_order 7) names
+#eval string_rsort (string_incresing_order 3) ["abc", "def", "ghi"]
+#eval string_rsort (string_incresing_order 4) ["ac", "deyz", "deyx"]
 
 
 end Chapter5
